Proofs/Form.thy
@@ -5,70 +5,70 @@ imports
   Semantics.IREval
 begin
 
-definition wff_start where
-  "wff_start g = (0 \<in> ids g \<and>
+definition wf_start where
+  "wf_start g = (0 \<in> ids g \<and>
     is_StartNode (kind g 0))"
 
-definition wff_closed where
-  "wff_closed g = 
+definition wf_closed where
+  "wf_closed g = 
     (\<forall> n \<in> ids g .
       inputs g n \<subseteq> ids g \<and>
       succ g n \<subseteq> ids g \<and>
       kind g n \<noteq> NoNode)"
 
-definition wff_phis where
-  "wff_phis g = 
+definition wf_phis where
+  "wf_phis g = 
     (\<forall> n \<in> ids g.
       is_PhiNode (kind g n) \<longrightarrow>
       length (ir_values (kind g n))
        = length (ir_ends 
            (kind g (ir_merge (kind g n)))))"
 
-definition wff_ends where
-  "wff_ends g = 
+definition wf_ends where
+  "wf_ends g = 
     (\<forall> n \<in> ids g .
       is_AbstractEndNode (kind g n) \<longrightarrow>
       card (usages g n) > 0)"
 
-text_raw \<open>\Snip{wff_graph}%\<close>
-fun wff_graph :: "IRGraph \<Rightarrow> bool" where
-  "wff_graph g = (wff_start g \<and> wff_closed g \<and> wff_phis g \<and> wff_ends g)"
+text_raw \<open>\Snip{wf_graph}%\<close>
+fun wf_graph :: "IRGraph \<Rightarrow> bool" where
+  "wf_graph g = (wf_start g \<and> wf_closed g \<and> wf_phis g \<and> wf_ends g)"
 text_raw \<open>\EndSnip\<close>
 
-lemmas wff_folds =
-  wff_graph.simps
-  wff_start_def
-  wff_closed_def
-  wff_phis_def
-  wff_ends_def
+lemmas wf_folds =
+  wf_graph.simps
+  wf_start_def
+  wf_closed_def
+  wf_phis_def
+  wf_ends_def
 
-fun wff_stamps :: "IRGraph \<Rightarrow> bool" where
-  "wff_stamps g = (\<forall> n \<in> ids g . 
+fun wf_stamps :: "IRGraph \<Rightarrow> bool" where
+  "wf_stamps g = (\<forall> n \<in> ids g . 
     (\<forall> v m . (g m \<turnstile> (kind g n) \<mapsto> v) \<longrightarrow> valid_value (stamp g n) v))"
 
-fun wff_stamp :: "IRGraph \<Rightarrow> (ID \<Rightarrow> Stamp) \<Rightarrow> bool" where
-  "wff_stamp g s = (\<forall> n \<in> ids g . 
+fun wf_stamp :: "IRGraph \<Rightarrow> (ID \<Rightarrow> Stamp) \<Rightarrow> bool" where
+  "wf_stamp g s = (\<forall> n \<in> ids g . 
     (\<forall> v m . (g m \<turnstile> (kind g n) \<mapsto> v) \<longrightarrow> valid_value (s n) v))"
 
-lemma wff_empty: "wff_graph start_end_graph"
-  unfolding start_end_graph_def wff_folds by simp
+lemma wf_empty: "wf_graph start_end_graph"
+  unfolding start_end_graph_def wf_folds by simp
 
-lemma wff_eg2_sq: "wff_graph eg2_sq"
-  unfolding eg2_sq_def wff_folds by simp
+lemma wf_eg2_sq: "wf_graph eg2_sq"
+  unfolding eg2_sq_def wf_folds by simp
 
 
-fun wff_values :: "IRGraph \<Rightarrow> bool" where
-  "wff_values g = (\<forall> n \<in> ids g .
-    (\<forall> v m . (g m \<turnstile> kind g n \<mapsto> v) \<longrightarrow> wff_value v))"
+fun wf_values :: "IRGraph \<Rightarrow> bool" where
+  "wf_values g = (\<forall> n \<in> ids g .
+    (\<forall> v m . (g m \<turnstile> kind g n \<mapsto> v) \<longrightarrow> wf_value v))"
 
-lemma wff_value_range:
-  "b > 1 \<and> b \<in> int_bits_allowed \<longrightarrow> {v. wff_value (IntVal b v)} = {v. ((-(2^(b-1)) \<le> v) \<and> (v < (2^(b-1))))}"
-  unfolding wff_value.simps
+lemma wf_value_range:
+  "b > 1 \<and> b \<in> int_bits_allowed \<longrightarrow> {v. wf_value (IntVal b v)} = {v. ((-(2^(b-1)) \<le> v) \<and> (v < (2^(b-1))))}"
+  unfolding wf_value.simps
   by auto
 
-lemma wff_value_bit_range:
-  "b = 1 \<longrightarrow> {v. wff_value (IntVal b v)} = {}"
-  unfolding wff_value.simps
+lemma wf_value_bit_range:
+  "b = 1 \<longrightarrow> {v. wf_value (IntVal b v)} = {}"
+  unfolding wf_value.simps
   by (simp add: int_bits_allowed_def)
 
 end
